vexview.py
@@ -1,0 +1,34 @@
+import sys
+from tig.symbolic_execution import get_project
+import json
+from tig.bininfo import Function
+
+with open("examples/RTOSDemo.elf.json", "r") as file:
+    data = json.load(file)
+
+if len(sys.argv) < 2:
+    function_name = "vTaskSwitchContext"
+    function_name = "xTimerIsTimerActive"
+else:
+    function_name = sys.argv[1]
+
+base_addr = data[0]["blocks"][0]["bb_start_vaddr"]
+p = get_project("examples/RTOSDemo.elf", base_addr)
+
+func = Function([x for x in data if x["function_name"] == function_name][0])
+
+
+def print_block_vex(block, insts):
+    isrb = p.factory.block(block.start_vaddr).vex
+    isrb.pp()
+    if isrb.next:
+        n_addr = isrb.next
+        while n_addr in insts:
+            isrb = p.factory.block(n_addr).vex
+            isrb.pp()
+            if isrb.next:
+                n_addr = isrb.next
+        
+for block in func.blocks:
+    print(block)
+    print_block_vex(block, [i.offset for i in block.instructions])
